examples/pseudo_bool/cp_encoding/cp_to_ilp_arrayScript.sml
@@ -8,10 +8,110 @@ Ancestors
   pbc cp ilp cp_to_ilp
 
 (* Element: Xs[Y - offset] = Z *)
+Definition encode_element_aux_1_def:
+  encode_element_aux_1 lb ub Y offset n =
+  let
+    lbc =
+      if lb < offset
+      then [mk_constraint_one_ge 1 Y offset]
+      else [];
+    ubc =
+      if ub > offset + n - 1
+      then [mk_constraint_one_ge (-1) Y (1 - n - offset)]
+      else []
+  in
+    lbc ++ ubc
+End
+
+Definition cencode_element_aux_1_def:
+  cencode_element_aux_1 lb ub Y offset n name =
+  let
+    lbann =
+      if lb < offset
+      then [mk_name name $ strlit"lb"]
+      else [];
+    ubann =
+      if ub > offset + n - 1
+      then [mk_name name $ strlit"ub"]
+      else []
+  in
+    List $ mk_annotate
+      (lbann ++ ubann)
+      (encode_element_aux_1 lb ub Y offset n)
+End
+
+Definition encode_element_aux_2_def:
+  encode_element_aux_2 bnd Xs Y Z offset n =
+  FLAT $ MAPi
+    (λi X.
+      [
+        bits_imply bnd [Pos $ INL (Eq Y $ offset + &i)] (mk_ge X Z);
+        bits_imply bnd [Pos $ INL (Eq Y $ offset + &i)] (mk_le X Z)
+      ])
+    Xs
+End
+
+Definition cencode_element_aux_2_def:
+  cencode_element_aux_2 bnd Xs Y Z offset n name =
+  List $ mk_annotate
+    (FLAT $ MAPi
+      (λi X.
+        [
+          mk_name name (int_to_string #"-" (&i) ^ strlit"ge");
+          mk_name name (int_to_string #"-" (&i) ^ strlit"le")
+        ])
+      Xs)
+    (encode_element_aux_2 bnd Xs Y Z offset n)
+End
+
+Definition cencode_element_def:
+  cencode_element bnd Xs Yi Z name ec =
+  let
+    len = LENGTH Xs;
+    (Y,offset) = Yi;
+    (lb,ub) =
+      case Y of
+        INL vY => bnd vY
+      | INR cY => (cY,cY);
+    (xs,ec') =
+      fold_cenc
+        (λi ec. cencode_full_eq bnd Y (offset + &i) ec)
+        (COUNT_LIST len)
+        ec
+  in
+    (Append
+      xs
+      (Append
+        (cencode_element_aux_1 lb ub Y offset (&len) name)
+        (cencode_element_aux_2 bnd Xs Y Z offset (&len) name)),
+    ec')
+End
+
 Definition encode_element_def:
   encode_element bnd Xs Yi Z =
-  [false_constr]
+  let
+    len = LENGTH Xs;
+    (Y,offset) = Yi;
+    (lb,ub) =
+      case Y of
+        INL vY => bnd vY
+      | INR cY => (cY,cY)
+  in
+    (FLAT $ GENLIST (λi. encode_full_eq bnd Y (offset + &i)) len) ++
+    ((encode_element_aux_1 lb ub Y offset (&len)) ++
+    (encode_element_aux_2 bnd Xs Y Z offset (&len)))
 End
+
+Theorem encode_element_aux_1[local]:
+  valid_assignment bnd wi ⇒
+  EVERY (λx. iconstraint_sem x (wi,reify_avar cs wi))
+    (FLAT (GENLIST
+      (λi. encode_full_eq bnd Y (offset + &i))
+      (LENGTH Xs)))
+Proof
+  rw[EVERY_FLAT,Once EVERY_MEM,MEM_GENLIST]>>
+  simp[encode_full_eq_sem,reify_avar_def,reify_reif_def]
+QED
 
 Theorem encode_element_sem_1:
   valid_assignment bnd wi ∧
@@ -19,7 +119,32 @@ Theorem encode_element_sem_1:
   EVERY (λx. iconstraint_sem x (wi,reify_avar cs wi))
     (encode_element bnd Xs Yi Z)
 Proof
-  cheat
+  PairCases_on ‘Yi’>>
+  rename1 ‘(Y,offset)’>>
+  Cases_on ‘Y’
+  >~[‘INL vY’]
+  >-(
+    rw[element_sem_def,mk_array_ind_def,
+      encode_element_def,encode_element_aux_1_def,encode_element_aux_2_def]>>
+    Cases_on ‘bnd vY’>>
+    simp[GSYM CONJ_ASSOC]>>
+    CONJ_TAC
+    >-simp[encode_element_aux_1]>>
+    rw[EVERY_FLAT,Once EVERY_MEM,MEM_MAPi,SF DNF_ss,reify_avar_def,reify_reif_def]>>
+    intLib.ARITH_TAC)
+  >~[‘INR cY’]
+  >-(
+    rw[encode_element_def]
+    >-simp[encode_element_aux_1]>>
+    fs[element_sem_def,mk_array_ind_def,varc_def]
+    >-(
+      rw[encode_element_aux_1_def,varc_def]>>
+      intLib.ARITH_TAC)
+    >-(
+      rw[encode_element_aux_2_def,EVERY_FLAT,
+        Once EVERY_MEM,MEM_FLAT,MEM_MAPi,SF DNF_ss,
+        reify_avar_def,reify_reif_def,varc_def]>>
+      intLib.ARITH_TAC))
 QED
 
 Theorem encode_element_sem_2:
@@ -28,7 +153,64 @@ Theorem encode_element_sem_2:
     (encode_element bnd Xs Yi Z) ⇒
   element_sem Xs Yi Z wi
 Proof
-  cheat
+  PairCases_on ‘Yi’>>
+  rename1 ‘element_sem _ (Y,offset) _ _’>>
+  Cases_on ‘Y’
+  >-(
+    rename1 ‘INL vY’>>
+    Cases_on ‘bnd vY’>>
+    strip_tac>>
+    gs[EVERY_FLAT,element_sem_def,mk_array_ind_def,encode_element_def,
+      MEM_FLAT,SF DNF_ss,EVERY_GENLIST]>>
+    simp[CONJ_ASSOC]>>
+    CONJ_ASM1_TAC
+    >-(
+      fs[encode_element_aux_1_def,valid_assignment_def,varc_def]>>
+      last_x_assum $ drule_then assume_tac>>
+      every_case_tac>>
+      fs[SF DNF_ss,varc_def]>>
+      intLib.ARITH_TAC)
+    >-(
+      fs[encode_element_aux_2_def,EVERY_FLAT,SF DNF_ss]>>
+      gvs[MEM_MAPi,SF DNF_ss,EVERY_MEM]>>
+      rpt (last_x_assum $ drule_then assume_tac)>>
+      intLib.ARITH_TAC))
+  >-(
+    strip_tac>>
+    gs[EVERY_FLAT,element_sem_def,mk_array_ind_def,encode_element_def,
+      MEM_FLAT,SF DNF_ss,EVERY_GENLIST]>>
+    simp[CONJ_ASSOC]>>
+    CONJ_ASM1_TAC
+    >-(
+      fs[encode_element_aux_1_def,varc_def]>>
+      every_case_tac>>
+      fs[SF DNF_ss,varc_def]>>
+      intLib.ARITH_TAC)
+    >-(
+      fs[encode_element_aux_2_def,EVERY_FLAT,SF DNF_ss]>>
+      gvs[MEM_MAPi,SF DNF_ss,EVERY_MEM]>>
+      rpt (last_x_assum $ drule_then assume_tac)>>
+      intLib.ARITH_TAC))
+QED
+
+Theorem cencode_element_sem:
+  valid_assignment bnd wi ∧
+  cencode_element bnd Xs Yi Z name ec = (es,ec') ⇒
+  enc_rel wi es (encode_element bnd Xs Yi Z) ec ec'
+Proof
+  PairCases_on ‘Yi’>>
+  rename1 ‘(Y,offset)’>>
+  rw[cencode_element_def,encode_element_def,UNCURRY_EQ]>>
+  simp[]>>
+  pure_rewrite_tac[GSYM APPEND_ASSOC]>>
+  irule enc_rel_Append>>
+  drule_at Any enc_rel_fold_cenc>>
+  gs[SYM MAP_COUNT_LIST]>>
+  disch_then $ irule_at Any>>
+  simp[enc_rel_encode_full_eq]>>
+  irule enc_rel_Append>>
+  simp[cencode_element_aux_1_def,cencode_element_aux_2_def]>>
+  metis_tac[enc_rel_List_mk_annotate]
 QED
 
 (* Element2D: Xss[Y1 - offset1][Y2 - offset2] = Z *)
